thys/Native_Word/Uint8.thy
@@ -164,14 +164,14 @@ code_printing code_module Uint8 \<rightharpoonup> (SML)
 val _ = if 3 <= Word.wordSize then () else raise (Fail ("wordSize less than 3"));
 
 structure Uint8 : sig
-  val set_bit : Word8.word -> IntInf.int -> bool -> Word8.word
+  val generic_set_bit : Word8.word -> IntInf.int -> bool -> Word8.word
   val shiftl : Word8.word -> IntInf.int -> Word8.word
   val shiftr : Word8.word -> IntInf.int -> Word8.word
   val shiftr_signed : Word8.word -> IntInf.int -> Word8.word
   val test_bit : Word8.word -> IntInf.int -> bool
 end = struct
 
-fun set_bit x n b =
+fun generic_set_bit x n b =
   let val mask = Word8.<< (0wx1, Word.fromLargeInt (IntInf.toLarge n))
   in if b then Word8.orb (x, mask)
      else Word8.andb (x, Word8.notb mask)
@@ -219,7 +219,7 @@ def less_eq(x: Byte, y: Byte) : Boolean =
     case false => y < 0 || x <= y
   }
 
-def set_bit(x: Byte, n: BigInt, b: Boolean) : Byte =
+def generic_set_bit(x: Byte, n: BigInt, b: Boolean) : Byte =
   b match {
     case true => (x | (1 << n.intValue)).toByte
     case false => (x & (1 << n.intValue).unary_~).toByte
@@ -416,7 +416,7 @@ global_interpretation uint8: word_type_copy_target_language Abs_uint8 Rep_uint8 
     and uint8_shiftl = uint8.shiftl
     and uint8_shiftr = uint8.shiftr
     and uint8_sshiftr = uint8.sshiftr
-    and uint8_set_bit = uint8.set_bit
+    and uint8_generic_set_bit = uint8.gen_set_bit
   by standard simp_all
 
 code_printing constant uint8_test_bit \<rightharpoonup>
@@ -425,11 +425,11 @@ code_printing constant uint8_test_bit \<rightharpoonup>
   (Scala) "Uint8.test'_bit" and
   (Eval) "(fn w => fn i => if i < 0 orelse i >= 8 then raise (Fail \"argument to uint8'_test'_bit out of bounds\") else Uint8.test'_bit w i)"
 
-code_printing constant uint8_set_bit \<rightharpoonup>
-  (SML) "Uint8.set'_bit" and
-  (Haskell) "Data'_Bits.setBitBounded" and
-  (Scala) "Uint8.set'_bit" and
-  (Eval) "(fn w => fn i => fn b => if i < 0 orelse i >= 8 then raise (Fail \"argument to uint8'_set'_bit out of bounds\") else Uint8.set'_bit w i b)"
+code_printing constant uint8_generic_set_bit \<rightharpoonup>
+  (SML) "Uint8.generic'_set'_bit" and
+  (Haskell) "Data'_Bits.genericSetBitBounded" and
+  (Scala) "Uint8.generic'_set'_bit" and
+  (Eval) "(fn w => fn i => fn b => if i < 0 orelse i >= 8 then raise (Fail \"argument to uint8'_generic'_set'_bit out of bounds\") else Uint8.generic'_set'_bit w i b)"
 
 code_printing constant uint8_shiftl \<rightharpoonup>
   (SML) "Uint8.shiftl" and
